Extend typing rules with assumptions context.
I have proved (hopefully) all lemmas about free variables and namings of
assumption contexts. But regularity and preservation are admitted for
now, as they need more lemmas about the behavior of the assumptions
context.

theories/base.v
@@ -59,22 +59,77 @@ Section set.
     set_solver.
   Qed.
 
+  #[global]
+  Instance set_Forall_proper :
+    Proper ((pointwise_relation _ iff) ==> (≡) ==> iff) (set_Forall (A:=A) (C:=C)).
+  Proof.
+    sfirstorder.
+  Qed.
+
 End set.
 
-(** * More Classes *)
+(** * Finite Set *)
 
 (** Polymorphic finite set *)
-Class PolyFinSet (S : forall A, EqDecision A -> Type) := {
-  poly_finset_elem_of :> forall A H, ElemOf A (S A H);
-  poly_finset_empty :> forall A H, Empty (S A H);
-  poly_finset_singleton :> forall A H, Singleton A (S A H);
-  poly_finset_union :> forall A H, Union (S A H);
-  poly_finset_intersection :> forall A H, Intersection (S A H);
-  poly_finset_difference :> forall A H, Difference (S A H);
-  poly_finset_elements :> forall A H, Elements A (S A H);
+Class PolyFinSet (M : Type -> Type) := {
+  poly_finset_elem_of A `{EqDecision A} :> ElemOf A (M A);
+  poly_finset_empty A `{EqDecision A} :> Empty (M A);
+  poly_finset_singleton A `{EqDecision A} :> Singleton A (M A);
+  poly_finset_union A `{EqDecision A} :> Union (M A);
+  poly_finset_intersection A `{EqDecision A} :> Intersection (M A);
+  poly_finset_difference A `{EqDecision A} :>Difference (M A);
+  poly_finset_elements A `{EqDecision A} :> Elements A (M A);
 
-  poly_finset :> forall A H, FinSet A (S A H);
+  poly_finset A `{EqDecision A} :> FinSet A (M A);
 }.
+
+Definition set_insert `{Singleton A C} `{Union C} (x : A) (X : C) : C := {[x]} ∪ X.
+
+Section map.
+
+  Context `{FinSet A C}.
+
+  Lemma set_map_id X : set_map (C:=C) id X ≡ X.
+  Proof.
+    set_solver.
+  Qed.
+
+  #[global]
+  Instance set_insert_proper : Proper ((=) ==> (≡) ==> (≡)) (set_insert (A:=A) (C:=C)).
+  Proof.
+    solve_proper.
+  Qed.
+
+  Lemma set_Forall_insert P (x : A) (X : C) :
+    set_Forall P (set_insert x X) <-> P x /\ set_Forall P X.
+  Proof.
+    unfold set_insert.
+    unfold set_Forall.
+    set_solver.
+  Qed.
+
+  Lemma set_Forall_insert_1 P (x : A) (X : C) :
+    set_Forall P (set_insert x X) -> P x /\ set_Forall P X.
+  Proof.
+    hauto use: set_Forall_insert.
+  Qed.
+
+  Lemma set_Forall_insert_2 (P : A -> Prop) (x : A) (X : C) :
+    P x -> set_Forall P X -> set_Forall P (set_insert x X).
+  Proof.
+    hauto use: set_Forall_insert.
+  Qed.
+
+  Context `{Set_ B D}.
+
+  Lemma set_map_insert (f : A -> B) (X : C) (x : A) :
+    set_map (D:=D) f (set_insert x X) ≡ set_insert (f x) (set_map (D:=D) f X).
+  Proof.
+    set_solver.
+  Qed.
+
+End map.
+
 
 (** * More Instances *)
 
