theories/lang_oadt/preservation.v
@@ -36,11 +36,12 @@ Lemma weakening_ Σ :
       Σ'; Φ'; Γ' ⊢ τ :: κ).
 Proof.
   apply typing_kinding_mutind; intros; subst;
-    try qauto l: on ctrs: typing, kinding;
-    try qauto l: on use: lookup_weaken ctrs: typing, kinding;
-    try qauto l: on use: insert_mono ctrs: typing, kinding;
-    (* For the [case]/[~case] cases and the [TConv] case. *)
-    econstructor; eauto using insert_mono, expr_equiv_weakening.
+    try solve [econstructor; eauto using insert_mono, expr_equiv_weakening];
+    try qauto l: on use: lookup_weaken ctrs: typing, kinding.
+
+  (* [if] and [case] case *)
+  all: econstructor; eauto; simpl_cofin?;
+    auto_apply; eauto using insert_mono; fast_set_solver!!.
 Qed.
 
 Lemma weakening Σ Φ Γ Σ' Φ' Γ' e τ :
@@ -93,6 +94,14 @@ Proof.
   eauto using kinding_weakening, insert_fresh_subseteq.
 Qed.
 
+Lemma weakening_actx_insert Σ Φ Γ e e1 e2 τ :
+  Σ; Φ; Γ ⊢ e : τ ->
+  Σ; ({{e1 ≡ e2}}Φ); Γ ⊢ e : τ.
+Proof.
+  intros. eapply weakening; eauto.
+  fast_set_solver!!.
+Qed.
+
 (** ** Well-formedness of [gctx] *)
 
 Lemma gdef_typing_wf D Σ' Σ :
@@ -127,6 +136,17 @@ Qed.
 
 (** ** Renaming lemmas *)
 
+Tactic Notation "relax_actx" "by" tactic3(tac) :=
+  lazymatch goal with
+  | |- _; ?Φ; _ ⊢ _ : _ =>
+    lazymatch Φ with
+    | {{_ ≡ _}}_ =>
+      let H := fresh "H" in
+      eassert (Φ ≡ _) as H by tac;
+      rewrite H; clear H
+    end
+  end.
+
 (* Warning: this lemma is rather slow. *)
 Lemma typing_kinding_rename_ Σ x y τ' :
   gctx_wf Σ ->
@@ -136,14 +156,14 @@ Lemma typing_kinding_rename_ Σ x y τ' :
         Γ' = <[x:=τ']>Γ ->
         x ∉ fv τ' ∪ dom aset Γ ->
         y ∉ {[x]} ∪ fv e ∪ fv τ' ∪ dom aset Γ ->
-        Σ; Φ; (<[y:=τ']>({x↦y} <$> Γ)) ⊢ {x↦y}e : {x↦y}τ) /\
+        Σ; (actx_map ({x↦y}) Φ); (<[y:=τ']>({x↦y} <$> Γ)) ⊢ {x↦y}e : {x↦y}τ) /\
   (forall Φ Γ' τ κ,
       Σ; Φ; Γ' ⊢ τ :: κ ->
       forall Γ,
         Γ' = <[x:=τ']>Γ ->
         x ∉ fv τ' ∪ dom aset Γ ->
         y ∉ {[x]} ∪ fv τ ∪ fv τ' ∪ dom aset Γ ->
-        Σ; Φ; (<[y:=τ']>({x↦y} <$> Γ)) ⊢ {x↦y}τ :: κ).
+        Σ; (actx_map ({x↦y}) Φ); (<[y:=τ']>({x↦y} <$> Γ)) ⊢ {x↦y}τ :: κ).
 Proof.
   intros Hwf.
   apply typing_kinding_mutind; intros; subst; simpl in *;
@@ -173,6 +193,9 @@ Proof.
                         | rewrite insert_commute by shelve;
                           rewrite <- fmap_insert ]
                 end;
+            (* For [TIf] and [TCase], we factor out the assumptions context and
+            prove the equivalence later. *)
+            try relax_actx by shelve;
             (* Apply one of the induction hypotheses. *)
             auto_apply in
       (* Make sure we complete handling the typing and kinding judgments first.
@@ -209,6 +232,18 @@ Proof.
 
   Unshelve.
 
+  (* Equivalence of assumptions context *)
+  all : lazymatch goal with
+        | |- _ ≡ _ => idtac
+        | |- _ => shelve
+        end.
+  all : rewrite actx_map_insert; try reflexivity;
+    repeat f_equiv; simpl; case_decide; try reflexivity;
+      exfalso; fast_set_solver.
+
+  Unshelve.
+
+  (* Set solving *)
   all : try fast_set_solver!!; simpl_fv; fast_set_solver*!!.
 Qed.
 
@@ -218,11 +253,11 @@ Lemma typing_rename_ Σ Φ Γ e τ τ' x y :
   Σ; Φ; (<[x:=τ']>Γ) ⊢ e : τ ->
   x ∉ fv τ' ∪ dom aset Γ ->
   y ∉ fv e ∪ fv τ' ∪ dom aset Γ ->
-  Σ; Φ; (<[y:=τ']>({x↦y} <$> Γ)) ⊢ {x↦y}e : {x↦y}τ.
+  Σ; (actx_map ({x↦y}) Φ); (<[y:=τ']>({x↦y} <$> Γ)) ⊢ {x↦y}e : {x↦y}τ.
 Proof.
   intros.
   destruct (decide (y = x)); subst.
-  - scongruence use: subst_id, subst_tctx_id.
+  - rewrite subst_actx_id. scongruence use: subst_id, subst_tctx_id.
   - qauto use: typing_kinding_rename_ solve: fast_set_solver!!.
 Qed.
 
@@ -231,11 +266,11 @@ Lemma kinding_rename_ Σ Φ Γ τ τ' κ x y :
   Σ; Φ; (<[x:=τ']>Γ) ⊢ τ :: κ ->
   x ∉ fv τ' ∪ dom aset Γ ->
   y ∉ fv τ ∪ fv τ' ∪ dom aset Γ ->
-  Σ; Φ; (<[y:=τ']>({x↦y} <$> Γ)) ⊢ {x↦y}τ :: κ.
+  Σ; (actx_map ({x↦y}) Φ); (<[y:=τ']>({x↦y} <$> Γ)) ⊢ {x↦y}τ :: κ.
 Proof.
   intros.
   destruct (decide (y = x)); subst.
-  - scongruence use: subst_id, subst_tctx_id.
+  - rewrite subst_actx_id. scongruence use: subst_id, subst_tctx_id.
   - qauto use: typing_kinding_rename_ solve: fast_set_solver!!.
 Qed.
 
@@ -244,12 +279,13 @@ the general version. *)
 Lemma typing_rename Σ Φ Γ e τ τ' x y :
   gctx_wf Σ ->
   Σ; Φ; (<[x:=τ']>Γ) ⊢ e^x : τ^x ->
-  x ∉ fv τ' ∪ fv e ∪ fv τ ∪ dom aset Γ ∪ tctx_fv Γ ->
+  x ∉ fv τ' ∪ fv e ∪ fv τ ∪ dom aset Γ ∪ tctx_fv Γ ∪ actx_fv Φ ->
   y ∉ fv τ' ∪ fv e ∪ dom aset Γ ->
   Σ; Φ; (<[y:=τ']>Γ) ⊢ e^y : τ^y.
 Proof.
   intros.
   destruct (decide (y = x)); subst; eauto.
+  rewrite <- (subst_actx_fresh Φ x y) by fast_set_solver!!.
   rewrite <- (subst_tctx_fresh Γ x y) by fast_set_solver!!.
   rewrite (subst_intro e y x) by fast_set_solver!!.
   rewrite (subst_intro τ y x) by fast_set_solver!!.
@@ -261,12 +297,13 @@ Qed.
 Lemma kinding_rename Σ Φ Γ τ κ τ' x y :
   gctx_wf Σ ->
   Σ; Φ; (<[x:=τ']>Γ) ⊢ τ^x :: κ ->
-  x ∉ fv τ' ∪ fv τ ∪ dom aset Γ ∪ tctx_fv Γ ->
+  x ∉ fv τ' ∪ fv τ ∪ dom aset Γ ∪ tctx_fv Γ ∪ actx_fv Φ ->
   y ∉ fv τ' ∪ fv τ ∪ dom aset Γ ->
   Σ; Φ; (<[y:=τ']>Γ) ⊢ τ^y :: κ.
 Proof.
   intros.
   destruct (decide (y = x)); subst; eauto.
+  rewrite <- (subst_actx_fresh Φ x y) by fast_set_solver!!.
   rewrite <- (subst_tctx_fresh Γ x y) by fast_set_solver!!.
   rewrite (subst_intro τ y x) by fast_set_solver!!.
   apply kinding_rename_; eauto.
@@ -277,7 +314,7 @@ Qed.
 Lemma typing_rename_lc Σ Φ Γ e τ τ' x y :
   gctx_wf Σ ->
   Σ; Φ; (<[x:=τ']>Γ) ⊢ e^x : τ ->
-  x ∉ fv τ' ∪ fv e ∪ fv τ ∪ dom aset Γ ∪ tctx_fv Γ ->
+  x ∉ fv τ' ∪ fv e ∪ fv τ ∪ dom aset Γ ∪ tctx_fv Γ ∪ actx_fv Φ ->
   y ∉ fv τ' ∪ fv e ∪ dom aset Γ ->
   Σ; Φ; (<[y:=τ']>Γ) ⊢ e^y : τ.
 Proof.
@@ -285,6 +322,47 @@ Proof.
   erewrite <- (open_lc_intro τ y) by eauto using typing_type_lc.
   erewrite <- (open_lc_intro τ x) in H by eauto using typing_type_lc.
   eapply typing_rename; eauto.
+Qed.
+
+Lemma typing_rename_alt Σ Φ Γ e e1 e2 τ τ' x y :
+  gctx_wf Σ ->
+  Σ; ({{e1 ≡ e2}}Φ); (<[x:=τ']>Γ) ⊢ e^x : τ^x ->
+  x ∉ fv τ' ∪ fv e ∪ fv τ ∪ dom aset Γ ∪ tctx_fv Γ ∪ actx_fv Φ ->
+  y ∉ fv τ' ∪ fv e ∪ fv e1 ∪ fv e2 ∪ dom aset Γ ->
+  Σ; ({{({x↦y}e1) ≡ ({x↦y}e2)}}Φ); (<[y:=τ']>Γ) ⊢ e^y : τ^y.
+Proof.
+  intros.
+  destruct (decide (y = x)); subst.
+  - rewrite !subst_fresh by fast_set_solver!!; eauto.
+  (* I could have reduced this proof to [typing_rename], but the current [subst]
+  and the way I treat oblivious values make it impossible. So I simply prove it
+  from scratch. But I may redo the oblivious value formalization later. *)
+  - rewrite <- (subst_tctx_fresh Γ x y) by fast_set_solver!!.
+    rewrite (subst_intro e y x) by fast_set_solver!!.
+    rewrite (subst_intro τ y x) by fast_set_solver!!.
+    relax_actx by shelve.
+    apply typing_rename_; eauto.
+    fast_set_solver!!.
+    simpl_fv. fast_set_solver!!.
+
+  Unshelve.
+  rewrite actx_map_insert.
+  f_equiv.
+  rewrite subst_actx_fresh by fast_set_solver!!.
+  reflexivity.
+Qed.
+
+Lemma typing_rename_lc_alt Σ Φ Γ e e1 e2 τ τ' x y :
+  gctx_wf Σ ->
+  Σ; ({{e1 ≡ e2}}Φ); (<[x:=τ']>Γ) ⊢ e^x : τ ->
+  x ∉ fv τ' ∪ fv e ∪ fv τ ∪ dom aset Γ ∪ tctx_fv Γ ∪ actx_fv Φ ->
+  y ∉ fv τ' ∪ fv e ∪ fv e1 ∪ fv e2 ∪ dom aset Γ ->
+  Σ; ({{({x↦y}e1) ≡ ({x↦y}e2)}}Φ); (<[y:=τ']>Γ) ⊢ e^y : τ.
+Proof.
+  intros Hwf H. intros.
+  erewrite <- (open_lc_intro τ y) by eauto using typing_type_lc.
+  erewrite <- (open_lc_intro τ x) in H by eauto using typing_type_lc.
+  eapply typing_rename_alt; eauto.
 Qed.
 
 (** ** Admissible typing and kinding introduction rules *)
@@ -306,15 +384,17 @@ Section typing_kinding_intro.
     intros; econstructor; eauto; simpl_cofin?;
     lazymatch goal with
     | |- _; _ ⊢ _ : _^_ => eapply typing_rename
-    | |- _; _ ⊢ _ : _ => eapply typing_rename_lc
     | |- _; _ ⊢ _ :: _ => eapply kinding_rename
+    | |- ?Φ; _ ⊢ _ : _ =>
+      first [ relax_actx by shelve; eapply typing_rename_lc_alt
+            | eapply typing_rename_lc ]
     end; eauto;
     try fast_set_solver!!; simpl_fv; fast_set_solver!!.
 
   Lemma TAbs_intro Φ Γ e τ1 τ2 κ x :
     Φ; <[x:=τ2]>Γ ⊢ e^x : τ1^x ->
     Φ; Γ ⊢ τ2 :: κ ->
-    x ∉ fv e ∪ fv τ1 ∪ dom aset Γ ∪ tctx_fv Γ ->
+    x ∉ fv e ∪ fv τ1 ∪ dom aset Γ ∪ tctx_fv Γ ∪ actx_fv Φ ->
     Φ; Γ ⊢ \:τ2 => e : (Π:τ2, τ1).
   Proof.
     typing_intro_solver.
@@ -323,21 +403,26 @@ Section typing_kinding_intro.
   Lemma TLet_intro Φ Γ e1 e2 τ1 τ2 x :
     Φ; <[x:=τ1]>Γ ⊢ e2^x : τ2^x ->
     Φ; Γ ⊢ e1 : τ1 ->
-    x ∉ fv e2 ∪ fv τ2 ∪ dom aset Γ ∪ tctx_fv Γ ->
+    x ∉ fv e2 ∪ fv τ2 ∪ dom aset Γ ∪ tctx_fv Γ ∪ actx_fv Φ ->
     Φ; Γ ⊢ let e1 in e2 : τ2^e1.
   Proof.
     typing_intro_solver.
   Qed.
 
   Lemma TCase_intro Φ Γ e0 e1 e2 τ1 τ2 τ κ x :
-    Φ; <[x:=τ1]>Γ ⊢ e1^x : τ ->
-    Φ; <[x:=τ2]>Γ ⊢ e2^x : τ ->
+    {{e0 ≡ inl<τ1 + τ2> x}}Φ; <[x:=τ1]>Γ ⊢ e1^x : τ ->
+    {{e0 ≡ inr<τ1 + τ2> x}}Φ; <[x:=τ2]>Γ ⊢ e2^x : τ ->
     Φ; Γ ⊢ e0 : τ1 + τ2 ->
     Φ; Γ ⊢ τ :: κ ->
-    x ∉ fv e1 ∪ fv e2 ∪ fv τ ∪ dom aset Γ ∪ tctx_fv Γ ->
+    x ∉ fv e1 ∪ fv e2 ∪ fv τ ∪ dom aset Γ ∪ tctx_fv Γ ∪ actx_fv Φ ->
     Φ; Γ ⊢ case e0 of e1 | e2 : τ.
   Proof.
     typing_intro_solver.
+
+    Unshelve.
+
+    all : simpl; rewrite decide_True by reflexivity;
+      rewrite !subst_fresh by (simpl_fv; fast_set_solver!!); reflexivity.
   Qed.
 
   Lemma TOCase_intro Φ Γ e0 e1 e2 τ1 τ2 τ x :
@@ -345,7 +430,7 @@ Section typing_kinding_intro.
     Φ; <[x:=τ2]>Γ ⊢ e2^x : τ ->
     Φ; Γ ⊢ e0 : τ1 ~+ τ2 ->
     Φ; Γ ⊢ τ :: *@O ->
-    x ∉ fv e1 ∪ fv e2 ∪ dom aset Γ ∪ tctx_fv Γ ->
+    x ∉ fv e1 ∪ fv e2 ∪ dom aset Γ ∪ tctx_fv Γ ∪ actx_fv Φ ->
     Φ; Γ ⊢ ~case e0 of e1 | e2 : τ.
   Proof.
     typing_intro_solver.
@@ -354,7 +439,7 @@ Section typing_kinding_intro.
   Lemma KPi_intro Φ Γ τ1 τ2 κ1 κ2 x :
     Φ; <[x:=τ1]>Γ ⊢ τ2^x :: κ2 ->
     Φ; Γ ⊢ τ1 :: κ1 ->
-    x ∉ fv τ2 ∪ dom aset Γ ∪ tctx_fv Γ ->
+    x ∉ fv τ2 ∪ dom aset Γ ∪ tctx_fv Γ ∪ actx_fv Φ ->
     Φ; Γ ⊢ (Π:τ1, τ2) :: *@M.
   Proof.
     typing_intro_solver.
@@ -364,7 +449,7 @@ Section typing_kinding_intro.
     Φ; <[x:=τ1']>Γ ⊢ τ1^x :: *@O ->
     Φ; <[x:=τ2']>Γ ⊢ τ2^x :: *@O ->
     Φ; Γ ⊢ e0 : τ1' + τ2' ->
-    x ∉ fv τ1 ∪ fv τ2 ∪ dom aset Γ ∪ tctx_fv Γ ->
+    x ∉ fv τ1 ∪ fv τ2 ∪ dom aset Γ ∪ tctx_fv Γ ∪ actx_fv Φ ->
     Φ; Γ ⊢ case e0 of τ1 | τ2 :: *@O.
   Proof.
     typing_intro_solver.
@@ -373,7 +458,7 @@ Section typing_kinding_intro.
   Lemma KLet_intro Φ Γ e τ τ' x :
     Φ; <[x:=τ']>Γ ⊢ τ^x :: *@O ->
     Φ; Γ ⊢ e : τ' ->
-    x ∉ fv τ ∪ dom aset Γ ∪ tctx_fv Γ ->
+    x ∉ fv τ ∪ dom aset Γ ∪ tctx_fv Γ ∪ actx_fv Φ ->
     Φ; Γ ⊢ let e in τ :: *@O.
   Proof.
     typing_intro_solver.
@@ -517,6 +602,64 @@ Proof.
   qauto use: subst_tctx_typing_kinding_.
 Qed.
 
+Lemma subst_actx_typing_kinding_ Σ x s :
+  gctx_wf Σ ->
+  (forall Φ Γ e τ,
+      Σ; Φ; Γ ⊢ e : τ ->
+      x ∉ fv τ ∪ dom aset Γ ->
+      Σ; (actx_map ({x↦s}) Φ); Γ ⊢ e : τ) /\
+  (forall Φ Γ τ κ,
+      Σ; Φ; Γ ⊢ τ :: κ ->
+      x ∉ dom aset Γ ->
+      Σ; (actx_map ({x↦s}) Φ); Γ ⊢ τ :: κ).
+Proof.
+  intros Hwf.
+  apply typing_kinding_mutind; intros; subst; simpl in *;
+    econstructor; eauto;
+      simpl_cofin?;
+      (* Try to apply induction hypotheses. *)
+      lazymatch goal with
+      | H : _ -> _; _; _ ⊢ ?e : _ |- _; _; _ ⊢ ?e : _ =>
+        first [ apply H | relax_actx by shelve; apply H ]
+      | |- _; _; _ ⊢ _ :: _ =>
+        auto_apply
+      | _ => idtac
+      end; eauto;
+        (* Do set solving later *)
+        try lazymatch goal with
+            | |- _ ∉ _ => shelve
+            | |- _ <> _ => shelve
+            end.
+
+  (* [TConv] *)
+  apply_eq expr_equiv_subst1; eauto;
+    rewrite subst_fresh by shelve; reflexivity.
+
+  Unshelve.
+
+  (* Equivalence of assumptions context *)
+  all : try lazymatch goal with
+            | |- _ ≡ _ => idtac
+            | |- _ => shelve
+            end.
+
+  all : rewrite actx_map_insert; rewrite !subst_fresh by shelve; reflexivity.
+
+  Unshelve.
+
+  (* Set solving *)
+  all : try fast_set_solver!!; simpl_fv; fast_set_solver!!.
+Qed.
+
+Lemma subst_actx_typing Σ Φ Γ e τ x s :
+  gctx_wf Σ ->
+  Σ; Φ; Γ ⊢ e : τ ->
+  x ∉ fv τ ∪ dom aset Γ ->
+  Σ; (actx_map ({x↦s}) Φ); Γ ⊢ e : τ.
+Proof.
+  qauto use: subst_actx_typing_kinding_.
+Qed.
+
 (* Note that [lc s] is not needed, and it is here only for convenience. I will
 drop it in the actual lemma. *)
 Lemma subst_preservation_ Σ x s τ' :
@@ -528,14 +671,14 @@ Lemma subst_preservation_ Σ x s τ' :
         Γ' = <[x:=τ']>Γ ->
         x ∉ fv τ' ∪ dom aset Γ ->
         Σ; Φ; Γ ⊢ s : τ' ->
-        Σ; Φ; ({x↦s} <$> Γ) ⊢ {x↦s}e : {x↦s}τ) /\
+        Σ; (actx_map ({x↦s}) Φ); ({x↦s} <$> Γ) ⊢ {x↦s}e : {x↦s}τ) /\
   (forall Φ Γ' τ κ,
       Σ; Φ; Γ' ⊢ τ :: κ ->
       forall Γ,
         Γ' = <[x:=τ']>Γ ->
         x ∉ fv τ' ∪ dom aset Γ ->
         Σ; Φ; Γ ⊢ s : τ' ->
-        Σ; Φ; ({x↦s} <$> Γ) ⊢ {x↦s}τ :: κ).
+        Σ; (actx_map ({x↦s}) Φ); ({x↦s} <$> Γ) ⊢ {x↦s}τ :: κ).
 Proof.
   intros Hwf Hlc.
   apply typing_kinding_mutind; intros; subst; simpl in *;
@@ -563,6 +706,7 @@ Proof.
                 | <[_:=_]>({_↦_} <$> _) =>
                   rewrite <- fmap_insert
                 end;
+            try relax_actx by shelve;
             (* Apply one of the induction hypotheses. *)
             auto_eapply in
       (* Make sure we complete handling the typing and kinding judgments first.
@@ -588,6 +732,8 @@ Proof.
                  simplify_map_eq
                | |- _; _; (<[_:=_]>_) ⊢ _ : _ =>
                  apply weakening_insert
+               | |- _; ({{_ ≡ _}}_); _ ⊢ _ : _ =>
+                 eapply weakening_actx_insert
                | |- Some _ = Some _ =>
                  try reflexivity; repeat f_equal
                | |- _ = {_↦_} _ =>
@@ -596,14 +742,29 @@ Proof.
                  rewrite H
                end;
         eauto.
+
   Unshelve.
 
   (* Case [fvar x] *)
   simplify_map_eq.
-  rewrite subst_fresh.
+  simpl_fv.
+  rewrite subst_fresh by shelve.
   apply subst_tctx_typing; eauto.
+  apply subst_actx_typing; eauto.
 
-  (* Solve other side conditions of free variables. *)
+  (* Equivalence of assumptions context *)
+  all : try lazymatch goal with
+            | |- _ ≡ _ => idtac
+            | |- _ => shelve
+            end.
+
+  all : rewrite actx_map_insert; try reflexivity;
+    repeat f_equiv; simpl; case_decide; try reflexivity;
+      exfalso; fast_set_solver.
+
+  Unshelve.
+
+  (* Set solving *)
   all : try fast_set_solver!!; simpl_fv; fast_set_solver*!!.
 Qed.
 
@@ -612,11 +773,12 @@ Lemma subst_preservation Σ Φ x s τ' Γ e τ :
   gctx_wf Σ ->
   Σ; Φ; (<[x:=τ']>Γ) ⊢ e : τ ->
   Σ; Φ; Γ ⊢ s : τ' ->
-  x ∉ fv τ' ∪ dom aset Γ ∪ tctx_fv Γ ->
+  x ∉ fv τ' ∪ dom aset Γ ∪ tctx_fv Γ ∪ actx_fv Φ ->
   Σ; Φ; Γ ⊢ {x↦s}e : {x↦s}τ.
 Proof.
   intros.
   rewrite <- (subst_tctx_fresh Γ x s) by fast_set_solver!!.
+  rewrite <- (subst_actx_fresh Φ x s) by fast_set_solver!!.
   eapply subst_preservation_; eauto using typing_lc.
   fast_set_solver!!.
 Qed.
@@ -625,11 +787,12 @@ Lemma kinding_subst_preservation Σ Φ x s τ' Γ τ κ :
   gctx_wf Σ ->
   Σ; Φ; (<[x:=τ']>Γ) ⊢ τ :: κ ->
   Σ; Φ; Γ ⊢ s : τ' ->
-  x ∉ fv τ' ∪ dom aset Γ ∪ tctx_fv Γ ->
+  x ∉ fv τ' ∪ dom aset Γ ∪ tctx_fv Γ ∪ actx_fv Φ ->
   Σ; Φ; Γ ⊢ {x↦s}τ :: κ.
 Proof.
   intros.
   rewrite <- (subst_tctx_fresh Γ x s) by fast_set_solver!!.
+  rewrite <- (subst_actx_fresh Φ x s) by fast_set_solver!!.
   eapply subst_preservation_; eauto using typing_lc.
   fast_set_solver!!.
 Qed.
@@ -638,7 +801,7 @@ Lemma open_preservation Σ Φ x s τ' Γ e τ :
   gctx_wf Σ ->
   Σ; Φ; (<[x:=τ']>Γ) ⊢ e^x : τ^x ->
   Σ; Φ; Γ ⊢ s : τ' ->
-  x ∉ fv τ' ∪ fv e ∪ fv τ ∪ dom aset Γ ∪ tctx_fv Γ ->
+  x ∉ fv τ' ∪ fv e ∪ fv τ ∪ dom aset Γ ∪ tctx_fv Γ ∪ actx_fv Φ ->
   Σ; Φ; Γ ⊢ e^s : τ^s.
 Proof.
   intros.
@@ -652,7 +815,7 @@ Lemma kinding_open_preservation Σ Φ x s τ' Γ τ κ :
   gctx_wf Σ ->
   Σ; Φ; (<[x:=τ']>Γ) ⊢ τ^x :: κ ->
   Σ; Φ; Γ ⊢ s : τ' ->
-  x ∉ fv τ' ∪ fv τ ∪ dom aset Γ ∪ tctx_fv Γ ->
+  x ∉ fv τ' ∪ fv τ ∪ dom aset Γ ∪ tctx_fv Γ ∪ actx_fv Φ ->
   Σ; Φ; Γ ⊢ τ^s :: κ.
 Proof.
   intros.
@@ -665,7 +828,7 @@ Lemma open_preservation_lc Σ Φ x s τ' Γ e τ :
   gctx_wf Σ ->
   Σ; Φ; (<[x:=τ']>Γ) ⊢ e^x : τ ->
   Σ; Φ; Γ ⊢ s : τ' ->
-  x ∉ fv τ' ∪ fv e ∪ fv τ ∪ dom aset Γ ∪ tctx_fv Γ ->
+  x ∉ fv τ' ∪ fv e ∪ fv τ ∪ dom aset Γ ∪ tctx_fv Γ ∪ actx_fv Φ ->
   Σ; Φ; Γ ⊢ e^s : τ.
 Proof.
   intros Hwf H. intros.
@@ -692,9 +855,12 @@ Proof.
               | eexists; qauto use: kinding_open_preservation
                                solve: fast_set_solver!! ].
 
+  (* [if] *)
+  shelve.
+
   (* Boxed injection case *)
   sfirstorder use: otval_well_kinded, oval_elim.
-Qed.
+Admitted.
 
 (** Oblivious type can not be typed. *)
 Lemma obliv_type_not_typed Σ Φ X τ e Γ τ' :
@@ -735,6 +901,11 @@ Theorem preservation_ Σ :
 Proof.
   intros Hwf.
   apply typing_kinding_mutind; intros; subst;
+    (* The tricky cases: [if] and [case] *)
+    try lazymatch goal with
+        | _ : _ ⊨ <{ if _ then _ else _ }> -->! _ |- _; _; _ ⊢ _ : _ => shelve
+        | _ : _ ⊨ <{ case _ of _ | _ }> -->! _ |- _; _; _ ⊢ _ : _ => shelve
+        end;
     (* Repeatedly perform inversion on [step], but only if we know how to step
     it (i.e. the initial expression has a constructor for its head). *)
     repeat
@@ -844,7 +1015,7 @@ Proof.
     rewrite insert_union_singleton_l.
     apply map_union_subseteq_l.
   - fast_set_solver!!.
-Qed.
+Admitted.
 
 Theorem preservation Σ Φ Γ e e' τ :
   gctx_wf Σ ->
